Continue tracking.

lean/privacy/tracking/coin.lean
@@ -1,13 +1,11 @@
-import privacy.transactions.transactions
-
-abbrev Transaction.ActionIdx (tx: Transaction) := Fin (tx.actions.length)
+import privacy.actions
 
 -- Map from action to optional (token, amount) pair.
 private abbrev CollectCoinsFunc := Action → Option (ℕ × ℕ)
 
-def Transaction.collect_coins (tx: Transaction) (f: CollectCoinsFunc) (token: ℕ) : List (tx.ActionIdx × ℕ) :=
-  tx.actions
-  |>.mapFinIdx (λ idx action h_idx ↦ ((⟨idx, h_idx⟩: tx.ActionIdx), action))
+def collect_coins (actions: List Action) (f: CollectCoinsFunc) (token: ℕ) : List (Fin actions.length × ℕ) :=
+  actions
+  |>.mapFinIdx (λ idx action h_idx ↦ ((⟨idx, h_idx⟩: Fin actions.length), action))
   |>.flatMap (λ (idx, action) ↦ (
     f action
     |>.filter (λ (token', _) ↦ token' = token)
@@ -15,17 +13,17 @@ def Transaction.collect_coins (tx: Transaction) (f: CollectCoinsFunc) (token: �
     |>.getD []
   ))
 
-theorem Transaction.collect_coins_length {tx: Transaction} {f: CollectCoinsFunc} {token: ℕ} :
-    (tx.collect_coins f token).length =
-    (tx.actions
+theorem collect_coins_length {actions: List Action} {f: CollectCoinsFunc} {token: ℕ} :
+    (collect_coins actions f token).length =
+    (actions
       |>.filterMap f
       |>.filter (λ (token', _) ↦ token' = token)
       |>.map (λ (_, amount) ↦ amount) |>.sum) := by
-  unfold Transaction.collect_coins
+  unfold collect_coins
   rw [List.length_flatMap]
   rw [List.map_congr_left (by
     intro ⟨idx, action⟩ h_idx_action
-    let g := λ a: tx.ActionIdx × Action ↦ (f a.2).map (λ val ↦ if val.1= token then val.2 else 0) |>.getD 0
+    let g := λ a: Fin actions.length × Action ↦ (f a.2).map (λ val ↦ if val.1= token then val.2 else 0) |>.getD 0
     show _ = g (idx, action)
     simp only [g]
     cases f action
@@ -40,8 +38,8 @@ theorem Transaction.collect_coins_length {tx: Transaction} {f: CollectCoinsFunc}
   rw [mapFinIdx_eq_map (λ action: Action ↦ (f action).map (λ val ↦ if val.1 = token then val.2 else 0) |>.getD 0)]
   simp [filter_map_sum_to_ite, filterMap_map_sum_to_getD]
 
-theorem Transaction.collect_coins_nodup {tx: Transaction} {f: CollectCoinsFunc} {token: ℕ} :
-    (tx.collect_coins f token).Nodup := by
+theorem collect_coins_nodup {actions: List Action} {f: CollectCoinsFunc} {token: ℕ} :
+    (collect_coins actions f token).Nodup := by
   apply mapFinIdx_flatMap_Nodup (j := λ (idx, x) ↦ idx)
   case g_nodup =>
     intro ⟨idx, action⟩
@@ -73,57 +71,3 @@ theorem Transaction.collect_coins_nodup {tx: Transaction} {f: CollectCoinsFunc} 
         rw [←h_res]
       case neg => simp [Option.filter_some, h] at h_res
     case none => simp [h_f] at h_res
-
-def Transaction.created_coins (tx: Transaction) (token: ℕ) : List (tx.ActionIdx × ℕ) :=
-  tx.collect_coins
-    (λ action ↦ (filter_CreateNote action).map (λ inp ↦ (inp.token, inp.amount)))
-    token
-
-def Transaction.canceled_coins (tx: Transaction) (token: ℕ) : List (tx.ActionIdx × ℕ) :=
-  tx.collect_coins
-   (λ action ↦ (filter_CancelNote action).map (λ inp ↦ (inp.token, inp.amount)))
-   token
-
-theorem created_coins_length (tx: Transaction) (token: ℕ) :
-    (tx.created_coins token).length = tx.sum_create_note_amounts token := by
-  unfold Transaction.created_coins
-  rw [tx.collect_coins_length]
-  simp only [Transaction₀.sum_create_note_amounts]
-  unfold Transaction₀.sum_amounts ActionFunc.create ActionFuncRes.from_create
-  simp only [List.filter_filterMap, List.map_filterMap]
-  apply congrArg
-  apply List.filterMap_congr
-  intro action h_actions
-  cases action
-  case CreateNote inp =>
-    by_cases h: inp.token = token
-    all_goals simp [h, Option.filter_some]
-
-  all_goals simp
-
-theorem canceled_coins_length (tx: Transaction) (token: ℕ) :
-    (tx.canceled_coins token).length = tx.sum_cancel_note_amounts token := by
-  unfold Transaction.canceled_coins
-  rw [tx.collect_coins_length]
-  simp only [Transaction₀.sum_cancel_note_amounts]
-  unfold Transaction₀.sum_amounts ActionFunc.cancel ActionFuncRes.from_cancel
-  simp only [List.filter_filterMap, List.map_filterMap]
-  apply congrArg
-  apply List.filterMap_congr
-  intro action h_actions
-  cases action
-  case CancelNote inp =>
-    by_cases h: inp.token = token
-    all_goals simp [h, Option.filter_some]
-
-  all_goals simp
-
--- A bijection between `created_coins.toFinset` and `canceled_coins.toFinset`.
-def Transaction.coins_equiv (tx: Transaction) (token: ℕ) :
-    (tx.created_coins token).toFinset ≃ (tx.canceled_coins token).toFinset :=
-  two_lists_equiv
-    (tx.created_coins token)
-    (tx.canceled_coins token)
-    (by rw [created_coins_length, canceled_coins_length, tx.h_balance])
-    collect_coins_nodup
-    collect_coins_nodup
