lean/privacy/tracking/tracking.lean
@@ -1,10 +1,82 @@
 import privacy.tracking.outgoing_notes
 import privacy.tracking.incoming_notes
+import privacy.tracking.coin
 
 theorem incoming_eq_outgoing
-  {crypto: Crypto} (stxs: SuccessfulTransactions crypto) (addr: ℕ) (token: ℕ) : false := by
-  have := outgoing_notes stxs addr token
-  conv at this => rhs; enter [1, 1, tx]; rw [tx.h_balance]
-  rw [←incoming_notes] at this
+  {crypto: Crypto} (stxs: SuccessfulTransactions crypto) (addr: ℕ) (token: ℕ) :
+  sum_cancel_note_amounts crypto stxs.rm addr token = (
+    create_note_actions crypto stxs.rm
+    |>.filter (λ inp ↦ inp.token = token ∧ inp.addralice = addr)
+    |>.map (λ inp ↦ inp.amount)
+    |>.sum
+  ) := by
+  rw [incoming_notes, outgoing_notes]
+  conv => rhs; enter [1, 1, tx]; rw [tx.h_balance]
 
-  sorry
+def created_coins (actions: List Action) (addralice token: ℕ) : List (Fin actions.length × ℕ) :=
+  collect_coins actions
+    (λ action ↦
+      filter_CreateNote action
+      |>.filter (λ inp ↦ inp.addralice = addralice)
+      |>.map (λ inp ↦ (inp.token, inp.amount))
+    )
+    token
+
+def canceled_coins (actions: List Action) (addrbob: ℕ) (token: ℕ) : List (Fin actions.length × ℕ) :=
+  collect_coins actions
+    (λ action ↦
+      filter_CancelNote action
+      |>.filter (λ inp ↦ inp.addrbob = addrbob)
+      |>.map (λ inp ↦ (inp.token, inp.amount))
+    )
+    token
+
+theorem created_coins_length {crypto: Crypto} (rm: ReachableMemory crypto) (addralice token: ℕ) :
+    (created_coins rm.actions addralice token).length = (
+      create_note_actions crypto rm
+      |>.filter (λ inp ↦ inp.token = token ∧ inp.addralice = addralice)
+      |>.map (λ inp ↦ inp.amount)
+      |>.sum
+    ) := by
+  unfold created_coins create_note_actions
+  rw [collect_coins_length]
+  simp only [List.filter_filterMap, List.map_filterMap]
+  apply congrArg
+  apply List.filterMap_congr
+  intro action h_actions
+  cases action
+  case CreateNote inp =>
+    by_cases h: inp.token = token
+    all_goals simp [h, Option.filter_some]
+    by_cases h: inp.addralice = addralice
+    all_goals simp [h, Option.filter_some]
+
+  all_goals simp
+
+theorem canceled_coins_length {crypto: Crypto} (rm: ReachableMemory crypto) (addrbob token: ℕ) :
+    (canceled_coins rm.actions addrbob token).length = sum_cancel_note_amounts crypto rm addrbob token := by
+  unfold canceled_coins sum_cancel_note_amounts cancel_note_actions
+  rw [collect_coins_length]
+
+  simp only [List.filter_filterMap, List.map_filterMap]
+  apply congrArg
+  apply List.filterMap_congr
+  intro action h_actions
+  cases action
+  case CancelNote inp =>
+    by_cases h: inp.token = token
+    all_goals simp [h, Option.filter_some]
+    by_cases h: inp.addrbob = addrbob
+    all_goals simp [h, Option.filter_some]
+
+  all_goals simp
+
+-- A bijection between `created_coins.toFinset` and `canceled_coins.toFinset`.
+def coins_equiv {crypto: Crypto} (stxs: SuccessfulTransactions crypto) (addr token: ℕ) :
+    (created_coins stxs.rm.actions addr token).toFinset ≃ (canceled_coins stxs.rm.actions addr token).toFinset :=
+  two_lists_equiv
+    (created_coins stxs.rm.actions addr token)
+    (canceled_coins stxs.rm.actions addr token)
+    (by rw [created_coins_length, canceled_coins_length, incoming_eq_outgoing])
+    collect_coins_nodup
+    collect_coins_nodup
